1) upgraded to 8.3pl1 2) changed to ProofGeneral 4.1, because CoqIDE 8.3 is slow 3) changed TV: some calls can be considered as normal commands, for example, calls that are added by Softbound, and whose behaviors are known. We call such calls 'libs'. With this change, each sub-block contains non-call cmds and libs, ends with other calls.
Admitted a lot of proofs about this new feature.



git-svn-id: https://webdav.seas.upenn.edu/svn/sol/vol@2801 eef5ea85-cc2e-0410-bd84-0fae1f012da8

src/Parser/main.ml
@@ -1,6 +1,5 @@
 open Printf
 open Llvm
-open Symexe_correct
 
 let debug = true
 
@@ -22,7 +21,8 @@ let main in_filename out_filename =
 
 	let coqom = Llvm2coq.translate_module debug ost om in
 			
-	eprintf "TV=%b\n" (tv_module coqim coqom);
+	eprintf "Eq TV=%b\n" (Eq_tv.tv_module coqim coqom);
+	eprintf "Sub TV=%b\n" (Sub_tv.tv_module coqim coqom);
 	
 	Coq2llvm.translate_module coqom;
 	
