src/Parser/myocamlbuild.ml
@@ -7,7 +7,10 @@ ocaml_lib ~extern:true "llvm_target";;
 ocaml_lib ~extern:true "llvm_bitreader";;
 ocaml_lib ~extern:true "llvm_bitwriter";;
 ocaml_lib ~extern:true "llvm_scalar_opts";;
-ocaml_lib ~extern:true "symexe_correct";;
+ocaml_lib ~extern:true "eq_tv";;
+ocaml_lib ~extern:true "sub_tv";;
+ocaml_lib ~extern:true "ssa_def";;
+ocaml_lib ~extern:true "ssa_lib";;
 
 flag ["link"; "ocaml"; "g++"] (S[A"-cc"; A"g++"]);;
 dep ["link"; "ocaml"; "use_bindings"] ;;
