src/TV/eq_tv.v
@@ -122,4 +122,11 @@ Ltac sumbool_simpl :=
   | [ H:is_true(tv_cmds _ _) |- _ ] => unfold is_true in H; apply sumbool2bool_true in H
   end.
 
+(*****************************)
+(*
+*** Local Variables: ***
+*** coq-prog-name: "coqtop" ***
+*** coq-prog-args: ("-emacs-U" "-I" "~/SVN/sol/vol/src/ssa/monads" "-I" "~/SVN/sol/vol/src/ssa/ott" "-I" "~/SVN/sol/vol/src/ssa/compcert" "-I" "~/SVN/sol/theory/metatheory_8.3") ***
+*** End: ***
+ *)
 
