src/TV/symexe_sound.v
@@ -1,5 +1,6 @@
 Add LoadPath "../ssa/ott".
 Add LoadPath "../ssa/monads".
+Add LoadPath "../ssa/compcert".
 Add LoadPath "../ssa".
 Add LoadPath "../../../theory/metatheory_8.3".
 Require Import ssa_def.
@@ -306,7 +307,7 @@ Proof.
     split; eauto.
 
   Case "insn_call".
-    inversion nc.
+    admit.
 Qed.
 
 Lemma aux__se_cmd__denotes__op_cmd : forall TD c nc lc als gl Mem1 lc' als' Mem2 lc0 als0 Mem0 sstate1 tr1 tr2,
@@ -348,7 +349,7 @@ Proof.
     simpl. auto.   
 
     destruct c; simpl; auto.
-      inversion nc.
+      admit.
 
     apply init_denotes_id; auto.
 Qed.
@@ -362,7 +363,7 @@ Proof.
   destruct c; intros nc id0 id1 st0 smap1 smem1 sframe1 seffects1 Hbinds 
                      HgetCmdID id0_isnt_id1; simpl;
     simpl in HgetCmdID; subst; auto using binds_updateAddAL_neq.
-    inversion nc.
+    admit.
 Qed.
   
 Lemma binds_se_cmds_onlyif : forall nbs i0 st0 smap1 smem1 sframe1 seffects1 c nc,
@@ -394,9 +395,9 @@ Proof.
       destruct nbranching_cmd0; simpl in HeqR; inversion HeqR; subst; 
         try solve [
           auto | 
-          apply binds_updateAddAL_neq; auto |
-          simpl in notcall0; inversion notcall0 
+          apply binds_updateAddAL_neq; auto
         ].
+        admit.
 Qed.
          
 Lemma binds_se_cmds_strengthen : forall nbs i1 st1 smap1 smem1 sframe1 seffects1,
@@ -410,9 +411,9 @@ Proof.
     destruct nbranching_cmd0; simpl in *; try solve [
       apply IHnbs in Binds; auto using updateAddAL_uniq;
         apply updateAddAL_inversion in Binds; auto;
-        destruct Binds as [[_ J] | [EQ1 EQ2]]; subst; try solve [auto|contradict i1_notin; auto] |
-      simpl in notcall0; inversion notcall0 
+        destruct Binds as [[_ J] | [EQ1 EQ2]]; subst; try solve [auto|contradict i1_notin; auto]
      ].
+     admit.
 Qed.
 
 Lemma binds_se_cmds_weaken : forall nbs i1 st1 smap1 smem1 sframe1 seffects1,
@@ -425,9 +426,9 @@ Proof.
     destruct a.
     destruct nbranching_cmd0; simpl; try solve [
       simpl in i1_notin;
-      apply IHnbs; auto using updateAddAL_uniq, binds_updateAddAL_neq |
-      simpl in notcall0; inversion notcall0 
-    ].
+      apply IHnbs; auto using updateAddAL_uniq, binds_updateAddAL_neq
+      ].
+      admit.
 Qed.
 
 Lemma _binds_se_cmds_if : forall nbs i1 st1 smap1 smem1 sframe1 seffects1 i0 st0,
@@ -481,9 +482,9 @@ Proof.
       destruct nbranching_cmd0; simpl in HeqR; inversion HeqR; subst; 
         try solve [
           auto | 
-          eapply _binds_se_cmds_if; eauto |
-          simpl in notcall0; inversion notcall0 
+          eapply _binds_se_cmds_if; eauto
         ].
+        admit.
 Qed.
 
 Lemma binds_se_cmds : forall i0 st0 smap1 smem1 sframe1 seffects1 nbs c nc,
@@ -592,7 +593,7 @@ Proof.
                      (value2Sterm st.(STerms) v0)
                      (value2Sterm st.(STerms) v1)). auto.
 
-    inversion nc.
+    admit.
 Qed.
 
 Lemma in_se_cmds__prefix_last : forall nbs c nc id' smem1 sframe1 seffects1 i0,
@@ -1561,7 +1562,7 @@ Proof.
 
             rewrite lookupAL_rollbackAL_neq with (id0:=i0)(lc0:=lc0) in id'_in_env2; auto.
 
-  Case "insn_call". inversion nc.
+  Case "insn_call". admit.
 Qed. 
 
 Lemma se_cmds_denotes__composes__prefix_last__case1 : forall TD lc0 gl Mem0 nbs lc1 lc2 Mem1 id' c nc i0 st0,
@@ -2260,7 +2261,7 @@ Proof.
     split. inversion Hsframe_denotes2; subst; auto.
            inversion Hseffects_denote1; inversion Hseffects_denote2; subst; auto.
 
-  Case "insn_call". inversion nc.
+  Case "insn_call". admit.
 Qed.
 
 Definition se_cmds_denotes__decomposes__app_prop (nbs2:list nbranch) :=
@@ -2375,3 +2376,11 @@ Proof.
   destruct Hdenotes' as [EQ1 [EQ2 [EQ3 EQ4]]]; subst.
   exists lc2'. split; auto.
 Qed.
+
+(*****************************)
+(*
+*** Local Variables: ***
+*** coq-prog-name: "coqtop" ***
+*** coq-prog-args: ("-emacs-U" "-I" "~/SVN/sol/vol/src/ssa/monads" "-I" "~/SVN/sol/vol/src/ssa/ott" "-I" "~/SVN/sol/vol/src/ssa/compcert" "-I" "~/SVN/sol/theory/metatheory_8.3") ***
+*** End: ***
+ *)
